# E. Negatives and Positives

## 题目信息

**时间限制**: 2 seconds
**内存限制**: 256 megabytes
**输入**: standard
**输出**: standard
**难度**: *1100
**标签**: dp, greedy, sortings

## 题目描述

Given an array $t$$a$ consisting of $t$$n$ elements, find the maximum possible sum the array can have after performing the following operation any number of times: Choose $t$$2$ adjacent elements and flip both of their signs. In other words choose an index $t$$i$ such that $t$$1 \leq i \leq n - 1$ and assign $t$$a_i = -a_i$ and $t$$a_{i+1} = -a_{i+1}$.

## 输入格式

The input consists of multiple test cases. The first line contains an integer $[-1, -1, -1]$$t$ ($[-1, -1, -1]$$1 \leq t \leq 1000$) — the number of test cases. The descriptions of the test cases follow.The first line of each test case contains an integer $[-1, -1, -1]$$n$ ($[-1, -1, -1]$$2 \leq n \leq 2\cdot10^5$) — the length of the array.The following line contains $[-1, -1, -1]$$n$ space-separated integers $[-1, -1, -1]$$a_1,a_2,\dots,a_n$ ($[-1, -1, -1]$$-10^9 \leq a_i \leq 10^9$).It is guaranteed that the sum of $[-1, -1, -1]$$n$ over all test cases does not exceed $[-1, -1, -1]$$2\cdot10^5$.

## 输出格式

For each test case, output the maximum possible sum the array can have after performing the described operation any number of times.

## 样例

### 样例 1

**输入:**
```
53-1 -1 -151 5 -5 0 231 2 36-1 10 9 8 7 62-1 -1
```

**输出:**
```
1
13
6
39
2
```

## 说明

For the first test case, by performing the operation on the first two elements, we can change the array from [−1,−1,−1][−1,−1,−1]$[-1, -1, -1]$ to [1,1,−1][1,1,−1]$[1, 1, -1]$, and it can be proven this array obtains the maximum possible sum which is 1+1+(−1)=11+1+(−1)=1$1 + 1 + (-1) = 1$.For the second test case, by performing the operation on −5−5$-5$ and 00$0$, we change the array from [1,5,−5,0,2][1,5,−5,0,2]$[1, 5, -5, 0, 2]$ to [1,5,−(−5),−0,2]=[1,5,5,0,2][1,5,−(−5),−0,2]=[1,5,5,0,2]$[1, 5, -(-5), -0, 2] = [1, 5, 5, 0, 2]$, which has the maximum sum since all elements are non-negative. So, the answer is 1+5+5+0+2=131+5+5+0+2=13$1 + 5 + 5 + 0 + 2 = 13$.For the third test case, the array already contains only positive numbers, so performing operations is unnecessary. The answer is just the sum of the whole array, which is 1+2+3=61+2+3=6$1 + 2 + 3 = 6$.
