# C. Minimizing the Sum

## 题目信息

**时间限制**: 2 seconds
**内存限制**: 256 megabytes
**输入**: standard
**输出**: standard
**难度**: *1700
**标签**: dp, implementation

## 题目描述

You are given an integer array a$t$$a$ of length n$t$$n$.You can perform the following operation: choose an element of the array and replace it with any of its neighbor's value.For example, if a=[3,1,2]$t$$a=[3, 1, 2]$, you can get one of the arrays [3,3,2]$t$$[3, 3, 2]$, [3,2,2]$t$$[3, 2, 2]$ and [1,1,2]$t$$[1, 1, 2]$ using one operation, but not [2,1,2$t$$[2, 1, 2$] or [3,4,2]$t$$[3, 4, 2]$. Your task is to calculate the minimum possible total sum of the array if you can perform the aforementioned operation at most k$t$$k$ times.

## 输入格式

The first line contains a single integer t$k$$t$ (1≤t≤104$k$$1 \le t \le 10^4$) — the number of test cases.The first line of each test case contains two integers n$k$$n$ and k$k$$k$ (1≤n≤3⋅105$k$$1 \le n \le 3 \cdot 10^5$; 0≤k≤10$k$$0 \le k \le 10$).The second line contains n$k$$n$ integers a1,a2,…,an$k$$a_1, a_2, \dots, a_n$ (1≤ai≤109$k$$1 \le a_i \le 10^9$).Additional constraint on the input: the sum of n$k$$n$ over all test cases doesn't exceed 3⋅105$k$$3 \cdot 10^5$.

## 输出格式

For each test case, print a single integer — the minimum possible total sum of the array if you can perform the aforementioned operation at most k$[3, 1, 2] \rightarrow [1, 1, 2$$k$ times.

## 样例

### 样例 1

**输入:**
```
43 13 1 21 354 22 2 1 36 34 1 2 2 4 3
```

**输出:**
```
4
5
5
10
```

## 说明

In the first example, one of the possible sequences of operations is the following: [3,1,2]→[1,1,2[3,1,2]→[1,1,2$[3, 1, 2] \rightarrow [1, 1, 2$].In the second example, you do not need to apply the operation.In the third example, one of the possible sequences of operations is the following: [2,2,1,3]→[2,1,1,3]→[2,1,1,1][2,2,1,3]→[2,1,1,3]→[2,1,1,1]$[2, 2, 1, 3] \rightarrow [2, 1, 1, 3] \rightarrow [2, 1, 1, 1]$.In the fourth example, one of the possible sequences of operations is the following: [4,1,2,2,4,3]→[1,1,2,2,4,3]→[1,1,1,2,4,3]→[1,1,1,2,2,3][4,1,2,2,4,3]→[1,1,2,2,4,3]→[1,1,1,2,4,3]→[1,1,1,2,2,3]$[4, 1, 2, 2, 4, 3] \rightarrow [1, 1, 2, 2, 4, 3] \rightarrow [1, 1, 1, 2, 4, 3] \rightarrow [1, 1, 1, 2, 2, 3]$.
